define SourceLang and give denotation

src/SourceLang.v
@@ -1,2 +1,189 @@
-Inductive expr :=
-|
+Require Import List.
+Import ListNotations.
+
+Inductive type_name :=
+| Bool
+| Nat
+| ListNat
+.
+
+Inductive type :=
+| ADT : type_name -> type
+| Arrow : type -> type -> type
+.
+
+(* a constructor that takes a list of arguments (with types given by the first index)
+   and returns a piece of data (with type given by the second index) *)
+Inductive constr : list type -> type -> Type :=
+| CTrue  : constr [] (ADT Bool)
+| CFalse : constr [] (ADT Bool)
+| CZero  : constr [] (ADT Nat)
+| CSucc  : constr [ADT Nat] (ADT Nat)
+| CNil   : constr [] (ADT ListNat)
+| CCons  : constr [ADT Nat; ADT ListNat] (ADT ListNat)
+.
+
+(* an eliminator that takes cases with types given by the first index,
+   eliminates a target with type given by the second index,
+   and produces a result with type given by the third index *)
+Inductive elim : list type -> type -> type -> Type :=
+| EBool : forall ty, elim [ty; ty] (ADT Bool) ty
+| ENat : forall ty, elim [ty; Arrow (ADT Nat) (Arrow ty ty)] (ADT Nat) ty
+| EListNat : forall ty, elim [ty; Arrow (ADT Nat) (Arrow (ADT ListNat) (Arrow ty ty))] (ADT ListNat) ty
+.
+
+(* heterogeneous lists. for more details see cpdt:
+   http://adam.chlipala.net/cpdt/html/Cpdt.DataStruct.html *)
+Inductive hlist {A : Type} (B : A -> Type) : list A -> Type :=
+| hnil : hlist B []
+| hcons : forall {a} (b : B a) l, hlist B l -> hlist B (a :: l)
+.
+Arguments hnil {A} {B}.
+Arguments hcons {A} {B} {a} b {l} h.
+
+Definition hhead {A B} {a : A} {l} (h : hlist B (a :: l)) : B a :=
+  match h in hlist _ l return match l with
+                              | [] => unit
+                              | x :: _ => B x
+                              end with
+  | hnil => tt
+  | hcons b _ => b
+  end.
+
+Definition htail {A B} {a : A} {l} (h : hlist B (a :: l)) : hlist B l :=
+  match h in hlist _ l return match l with
+                              | [] => unit
+                              | _ :: l' => hlist B l'
+                              end with
+  | hnil => tt
+  | hcons _ t => t
+  end.
+
+
+(* `member` is isomorphic to `In`, but its proof-relevant, so it can be used as data.
+   this is used below to represent variables as dependent de Bruijn indices. *)
+Inductive member {A : Type} (a : A) : list A -> Type :=
+| Here : forall l, member a (a :: l)
+| There : forall x l, member a l -> member a (x :: l)
+.
+Arguments Here {A} {a} {l}.
+Arguments There {A} {a} {x} {l} m.
+
+(* given an index into l, lookup the corresponding element in an (hlist l) *)
+Fixpoint hget {A B} {l : list A} (h : hlist B l) (x : A) {struct h} : member x l -> B x :=
+    match h with
+    | hnil =>
+      fun m : member x [] =>
+        match m in member _ l0 return match l0 with
+                                      | nil => B x
+                                      | _ :: _ => unit
+                                      end with
+        | Here => tt
+        | There _ => tt
+        end
+    | @hcons _ _ a b l' h' =>
+      fun m : member x (a :: l') =>
+        match m in member _ l0 return match l0 with
+                                      | nil => unit
+                                      | a'' :: l'' => B a'' -> (member x l'' -> B x) -> B x
+                                      end with
+        | Here => fun b' _ => b'
+        | There m' => fun _ rec => rec m'
+        end b (hget h' x)
+    end.
+Arguments hget {A B l} h {x} m.
+
+
+Section expr.
+(* since this type makes hlists of recursive calls, the auto-generated schemes are garbage. *)
+Local Unset Elimination Schemes.
+Inductive expr : list type -> type -> Type :=
+| Var : forall {ty l}, member ty l -> expr l ty
+| Lam : forall {ty1 ty2 l}, expr (ty1 :: l) ty2 -> expr l (Arrow ty1 ty2)
+| App : forall {ty1 ty2 l}, expr l (Arrow ty1 ty2) -> expr l ty1 -> expr l ty2
+| Constr : forall {ty arg_tys l} (c : constr arg_tys ty), hlist (expr l) arg_tys -> expr l ty
+| Elim : forall {case_tys target_ty ty l} (e : elim case_tys target_ty ty),
+    hlist (expr l) case_tys ->
+    expr l target_ty ->
+    expr l ty
+.
+End expr.
+
+Definition type_name_denote (tyn : type_name) : Type :=
+  match tyn with
+  | Bool => bool
+  | Nat => nat
+  | ListNat => list nat
+  end.
+
+Fixpoint type_denote (ty : type) : Type :=
+  match ty with
+  | ADT tyn => type_name_denote tyn
+  | Arrow ty1 ty2 => type_denote ty1 -> type_denote ty2
+  end.
+
+
+Definition constr_denote {arg_tys ty} (c : constr arg_tys ty) :
+  hlist type_denote arg_tys -> type_denote ty :=
+  match c with
+  | CTrue => fun _ => true
+  | CFalse => fun _ => false
+  | CZero => fun _ => 0
+  | CSucc => fun h => S (hhead h)
+  | CNil => fun _ => []
+  | CCons => fun h => cons (hhead h) (hhead (htail h))
+  end.
+
+
+Definition elim_denote {case_tys target_ty ty} (e : elim case_tys target_ty ty) :
+  hlist type_denote case_tys -> type_denote target_ty -> type_denote ty :=
+  match e with
+  | EBool _ => fun cases target => (bool_rect _ (hhead cases) (hhead (htail cases)) target)
+  | ENat _ => fun cases target => (nat_rect _ (hhead cases) (hhead (htail cases)) target)
+  | EListNat _ => fun cases target => (list_rect _ (hhead cases) (hhead (htail cases)) target)
+  end.
+
+
+Definition expr_denote {l ty} (e : expr l ty) (h : hlist type_denote l) : type_denote ty :=
+  let fix go {l ty} (e : expr l ty) (h : hlist type_denote l) : type_denote ty :=
+      let fix go_hlist {l tys} (es : hlist (expr l) tys) (h : hlist type_denote l) : hlist type_denote tys :=
+          match es in hlist _ tys0 return hlist _ tys0 with
+          | hnil  => hnil
+          | hcons e es' => hcons (go e h) (go_hlist es' h)
+          end
+      in match e in expr l0 ty0 return hlist type_denote l0 -> type_denote ty0 with
+         | Var m => fun h => hget h m
+         | Lam body => fun h x => go body (hcons x h)
+         | App f a => fun h => (go f h) (go a h)
+         | Constr c args => fun h => constr_denote c (go_hlist args h)
+         | Elim e cases target => fun h => elim_denote e (go_hlist cases h) (go target h)
+         end h
+  in go e h.
+
+
+Eval compute in expr_denote (Constr CTrue hnil) hnil.
+
+Eval compute in expr_denote (Lam(ty1 := ADT Bool) (Var Here)) hnil.
+
+Definition map_reflect {l} : expr l (Arrow (Arrow (ADT Nat) (ADT Nat)) (Arrow (ADT ListNat) (ADT ListNat))) :=
+  Lam
+  (Lam
+  (Elim (EListNat _)
+        (hcons (Constr CNil hnil)
+         (hcons
+          (Lam (Lam (Lam
+           (Constr CCons
+            (hcons
+              (App
+                (Var (There (There (There (There Here)))))
+                (Var (There (There Here))))
+             (hcons (Var Here) hnil))))))
+          hnil))
+        (Var Here))).
+
+
+Eval compute in expr_denote map_reflect hnil.
+Eval compute in @map nat nat.
+
+Example map_reflect_correct : forall l h, expr_denote(l := l) map_reflect h = @map nat nat.
+Proof. reflexivity. Qed.
